Add 'memory' to the non-informative event
Notice that this commit implements the following design decision:
The *whole* memory is emitted on the trace (at border states), and
the idea is that the trace relation will constrain only the
shared part of the memory. This design decision is crucial;
it allows us to avoid *computing* reachability and to instead
characterize the shared memory as a reachable part of the memory
that is given by just an inductive definition.

Notice also that as a result of emitting memory (whether the whole
memory or just the shared part) on the trace, the type of
trace events is now no longer an equality type.
This loss of decidable equality is not very catastrophic: after all,
we won't need it that much because the top-level theorems
and many lemmas will now be stated in terms of the trace relation
(that is not equality).

Some lemmas (like determinacy) will still need to be stated in terms
of decidable equality so that they remain conveniently usable.
(TODO: Check if it is possible to re-gain decidable equality in the
existence of memory on the trace event. Can we decide equality on
Memory.t?)

Common/Traces.v
@@ -55,9 +55,9 @@ Fixpoint well_bracketed_trace s t : bool :=
   | e :: t' =>
     (cur_comp s == cur_comp_of_event e) &&
     match e with
-    | ECall C _ _ C' =>
+    | ECall C _ _ _ C' =>
       well_bracketed_trace (StackState C' (C :: callers s)) t'
-    | ERet C _ C' =>
+    | ERet C _ _ C' =>
       match callers s with
       | [] => false
       | head :: tail =>
@@ -69,8 +69,8 @@ Fixpoint well_bracketed_trace s t : bool :=
 
 Definition run_event s e :=
   match e with
-  | ECall C _ _ C' => StackState C' (C :: callers s)
-  | ERet  C _   C' => StackState C' (tail (callers s))
+  | ECall C _ _ _ C' => StackState C' (C :: callers s)
+  | ERet  C _ _   C' => StackState C' (tail (callers s))
   (*| _ => s*)
   end.
 
@@ -84,12 +84,11 @@ Lemma well_bracketed_trace_cat s t1 t2 :
   well_bracketed_trace s t1 &&
   well_bracketed_trace (run_trace s t1) t2.
 Proof.  
-(* TODO: Try to understand and fix the proof. *)
-elim: t1 s=> [//|[C ? ? C'|C ? C'(*|? ? ?|? ? ?*)] t1 IH] [Ccur callers] /=.
+elim: t1 s=> [//|[C ? ? ? C'|C ? ? C'(*|? ? ?|? ? ?*)] t1 IH] [Ccur callers] /=.
   by rewrite IH andbA.
 case: eqP callers => [_ {Ccur}|_] //= [|top callers] //=.
   by rewrite IH andbA.
-Admitted.
+Qed.
 
 Definition seq_of_stack_state s := cur_comp s :: callers s.
 
@@ -101,9 +100,8 @@ Proof. by case=> [??] [??] [-> ->]. Qed.
 Lemma well_bracketed_trace_suffix t C C' Cs :
   well_bracketed_trace stack_state0 t ->
   suffix [:: C, C' & Cs] (run_trace stack_state0 t) ->
-  exists t1 P arg t2, t = t1 ++ ECall C' P arg C :: t2.
+  exists t1 P arg mem t2, t = t1 ++ ECall C' P arg mem C :: t2.
 Proof.
-(* TODO: Try to understand and fix the proof. *)
 set s0 := stack_state0.
 elim/last_ind: t=> [|t e IH] //=.
   by rewrite suffix_cons suffix_nil /= orbF => _ /eqP.
@@ -111,27 +109,27 @@ have -> : well_bracketed_trace s0 (rcons t e) =
           well_bracketed_trace s0 t &&
           well_bracketed_trace (run_trace s0 t) [:: e].
   by rewrite -cats1 well_bracketed_trace_cat andbC.
-rewrite run_trace1; case: e => [C1 P arg C2|C1 ? C2(*|? ? ?|? ? ?*)] /=.
+rewrite run_trace1; case: e => [C1 P arg mem C2|C1 ? ? C2(*|? ? ?|? ? ?*)] /=.
   rewrite andbT; case/andP=> wb_t /eqP <- {C1} /=.
   rewrite -[_ :: callers _]/(run_trace s0 t : seq _) suffix_cons /=.
   case/orP=> [/eqP|Hsuff].
     case: (run_trace _ _)=> [? ?] [<- <- <-] /=.
-    by eexists t, _, _, [::]; rewrite cats1.
-  case/(_ wb_t Hsuff): IH=> [t1 [P' [arg' [t2 ->]]]].
-  by eexists t1, P', arg', (rcons t2 _); rewrite rcons_cat; split; eauto.
+    by eexists t, _, _, _, [::]; rewrite cats1.
+  case/(_ wb_t Hsuff): IH=> [t1 [P' [arg' [mem' [t2 ->]]]]].
+  by eexists t1, P', arg', mem', (rcons t2 _); rewrite rcons_cat; split; eauto.
 case/and3P=> wb_t /eqP e1 e2.
 have -> : StackState C2 (tl (callers (run_trace s0 t))) =
           callers (run_trace s0 t) :> seq _.
   by case: (callers _) e2=> [|e cs] //= /andP [/eqP ->].
 move=> Hsuff; have {Hsuff} Hsuff: suffix [:: C, C' & Cs] (run_trace s0 t).
   by rewrite suffix_cons Hsuff orbT.
-case/(_ wb_t Hsuff): IH=> [t1 [P [arg [t2 ->]]]].
-  by eexists t1, P, arg, (rcons _ _); rewrite rcons_cat.
-Admitted.
+case/(_ wb_t Hsuff): IH=> [t1 [P [arg [mem [t2 ->]]]]].
+  by eexists t1, P, arg, mem, (rcons _ _); rewrite rcons_cat.
+Qed.
 
-Lemma well_bracketed_trace_inv t C res C' :
-  well_bracketed_trace stack_state0 (t ++ [:: ERet C res C']) ->
-  exists t1 P arg t2, t = t1 ++ ECall C' P arg C :: t2.
+Lemma well_bracketed_trace_inv t C res mem C' :
+  well_bracketed_trace stack_state0 (t ++ [:: ERet C res mem C']) ->
+  exists t1 P arg mem' t2, t = t1 ++ ECall C' P arg mem' C :: t2.
 Proof.
 rewrite -[t]cat0s.
 elim: t {1 3}nil=> [|e t IH] pre //=; last first.
@@ -153,8 +151,8 @@ Qed.
    performs is a possible read/write.  *)
 Definition well_formed_event intf (e: event) : bool :=
   match e with
-  | ECall C P _ C' => (C != C') && imported_procedure_b intf C C' P
-  | ERet  C _   C' => (C != C')
+  | ECall C P _ _ C' => (C != C') && imported_procedure_b intf C C' P
+  | ERet  C _ _   C' => (C != C')
   (*| ERead _ _ _ => false
   | EWrite _ _ _ => false*)
   end.
@@ -172,9 +170,11 @@ Lemma well_formed_trace_int intf t :
   closed_interface intf ->
   all (declared_event_comps intf) t.
 Proof.
+  (* [DynShare] TODO: The proof below works only if event is an equality type.
+     The reason for that is that "allP" relies on this fact.
+   *)
 Admitted.
-(*
-case/andP=> wb wf clos; rewrite /declared_event_comps.
+(*case/andP=> wb wf clos; rewrite /declared_event_comps.
 apply/allP; case=> [C P v C'|C v C'] /=; rewrite !mem_domm.
 - move/(allP wf)=> /andP [_ imp].
   move: (imp); rewrite /imported_procedure_b; case: getm => //= _ _.
@@ -187,6 +187,6 @@ apply/allP; case=> [C P v C'|C v C'] /=; rewrite !mem_domm.
   case/andP=> _ imp.
   case/imported_procedure_iff/clos: (imp)=> ? [-> _] /=.
   by move: imp; rewrite /imported_procedure_b; case: getm.
-Qed.
-*)
+Qed.*)
+
 End Traces.
